examples/conceptual/AssnsLemmaThmEtc.thy
@@ -13,12 +13,20 @@ print_doc_items
 section\<open>Definitions, Lemmas, Theorems, Assertions\<close>
 
 
-text*[aa::F, property = "[@{term ''True''}]"]\<open>Our definition of the HOL-Logic has the following properties:\<close>
+text*[aa::F, property = "[@{termrepr ''True''}]"]\<open>Our definition of the HOL-Logic has the following properties:\<close>
 assert*[aa::F] "True"
+
+ML\<open>  val (Const _ $ t $ t') =  @{docitem_attribute property :: aa}\<close>
 
 ML\<open>  ISA_core.property_list_dest  @{docitem_attribute property :: aa}\<close>
 
-assert*[aa::F] "True --> True" (* small pb: unicodes crashes here ... *)
+assert*[aa::F] "True \<longrightarrow> True" (* small pb: unicodes crashes here ... *)
+
+ML\<open>
+Syntax.read_term_global @{theory} "[@{term '' 'True @<longrightarrow> True' ''}]";
+
+@{term "[@{term '' ' True @<longrightarrow> True ' ''}]"} 
+\<close>
 
 ML\<open> ISA_core.property_list_dest @{docitem_attribute property :: aa}\<close>
 
